src/Enumeration/Iterators.dfy
@@ -6,7 +6,7 @@ module IteratorExperiments {
   import opened Frames
 
   iterator ForEachWithIndex<T(0)>(s: seq<T>) yields (element: T, index: nat)
-    ensures elements <= s
+    ensures elements == s
     yield ensures elements <= s
   {
     for i := 0 to |s|
@@ -21,29 +21,51 @@ module IteratorExperiments {
 
     method MoveNext() returns (more: bool)
       requires Valid()
+      requires !Done()
       modifies Repr
-      ensures fresh(Repr - old(Repr))
-      ensures more ==> Valid()
-      ensures more ==> Decreases() < old(Decreases())
+      decreases Repr
+      ensures ValidAndDisjoint()
+      ensures more <==> !Done()
+      ensures !Done() ==> Decreases() < old(Decreases())
 
     function method Current(): T
       reads this, Repr
       requires Valid()
+      requires !Done()
 
+    predicate Done()
+      requires Valid()
+      reads this, Repr
+
+    // Needs a better name, it's only a measure that is USED
+    // in decreases clauses but not the same thing.
+    // Although decreases is already overloaded to mean slightly
+    // different things for a method spec vs. a while loop spec.
+    // NOT what decreases means on an iterator though.
     function Decreases(): nat 
       reads this, Repr
       requires Valid()
+
+    // Should this be forced on every enumerator? Or provided on
+    // an Enumerator<T> wrapper instead, since it's implementable generically?
+    // ghost var enumerated: set<T>
   }
 
   class ForEachWithIndexEnumerator<T(0)> extends Enumerator<(T, nat)> {
 
     const iter: ForEachWithIndex<T>
     ghost var remaining: nat
+    ghost var done: bool
 
-    constructor(s: seq<T>) ensures Valid() ensures fresh(Repr) {
+    constructor(s: seq<T>) 
+      ensures Valid() 
+      ensures fresh(Repr) 
+      ensures !Done()
+    {
       iter := new ForEachWithIndex(s);
       new;
-      remaining := |iter.s|;
+      done := false;
+      remaining := |iter.s| - |iter.elements|;
       Repr := {this, iter};
     }
 
@@ -56,21 +78,28 @@ module IteratorExperiments {
       && iter._modifies <= Repr
       && iter._reads <= Repr
       && iter._new <= Repr
-      && iter.Valid()
+      && (!done ==> iter.Valid())
       && remaining == |iter.s| - |iter.elements|
+    }
+
+    predicate Done()
+      requires Valid()
+      reads this, Repr
+    {
+      done
     }
 
     method MoveNext() returns (more: bool) 
       requires Valid()
+      requires !Done()
       modifies Repr
-      ensures fresh(Repr - old(Repr))
-      ensures more ==> Valid()
-      ensures more ==> Decreases() < old(Decreases())
+      decreases Repr
+      ensures ValidAndDisjoint()
+      ensures more <==> !Done()
+      ensures !Done() ==> Decreases() < old(Decreases())
     {
       more := iter.MoveNext();
-      if (more) {
-        assert old(iter.elements) < iter.elements;
-      }
+      done := !more;
       remaining := |iter.s| - |iter.elements|;
       Repr := {this, iter} + iter._modifies + iter._reads + iter._new;
     }
@@ -82,10 +111,83 @@ module IteratorExperiments {
       (iter.element, iter.index)
     }
 
-    function Decreases(): nat reads this, Repr requires Valid() {
+    function Decreases(): nat 
+      reads this, Repr 
+      requires Valid() 
+    {
       remaining
     }
   }
+
+  // class Filter<T(0)> extends Enumerator<T> {
+  //   const wrapped: Enumerator<T>
+  //   const filter: T -> bool
+  //   var current: T
+
+  //   constructor(wrapped: Enumerator<T>, filter: T -> bool) 
+  //     requires wrapped.Valid()
+  //     ensures Valid() 
+  //   {
+  //     this.wrapped := wrapped;
+  //     this.filter := filter;
+  //     Repr := {this} + wrapped.Repr;
+  //   }
+
+  //   predicate Valid() reads this, Repr ensures Valid() ==> this in Repr {
+  //     && this in Repr
+  //     && ValidComponent(wrapped)
+  //   }
+
+  //   predicate Done()
+  //     requires Valid()
+  //     reads this, Repr
+  //   {
+  //     wrapped.Done()
+  //   }
+
+  //   method MoveNext() returns (more: bool) 
+  //     requires Valid()
+  //     requires !Done()
+  //     modifies Repr
+  //     decreases Repr
+  //     ensures ValidAndDisjoint()
+  //     ensures more <==> !Done()
+  //     ensures !Done() ==> Decreases() < old(Decreases())
+  //   {
+  //     more := true;
+  //     while (true)
+  //       invariant Valid()
+  //       invariant old(allocated(wrapped)) && fresh(wrapped.Repr - old(wrapped.Repr))
+  //       decreases more, wrapped.Decreases()
+  //     {
+  //       assert wrapped.Repr < Repr;
+  //       assert !wrapped.Done();
+  //       more := wrapped.MoveNext();
+  //       Repr := Repr + wrapped.Repr;
+
+  //       if (!more) { break; }
+
+  //       current := wrapped.Current();
+  //       if (filter(current)) {
+  //         break;
+  //       }
+  //     }
+  //   }
+
+  //   function method Current(): T
+  //     reads this, Repr
+  //     requires Valid()
+  //   {
+  //     current
+  //   }
+
+  //   function Decreases(): nat 
+  //     reads this, Repr
+  //     requires Valid() 
+  //   {
+  //     wrapped.Decreases()
+  //   }
+  // }
 
   method Main() {
     var s: seq<nat> := [1, 1, 2, 3, 5, 8];
@@ -95,15 +197,36 @@ module IteratorExperiments {
     var more := true;
     while (true) 
       invariant e.Valid()
+      invariant more <==> !e.Done()
       invariant old@start(allocated(e)) && fresh(e.Repr)
       decreases e.Decreases()
     {
       more := e.MoveNext();
       if (!more) { break; }
-
       var (element, index) := e.Current();
+
       print "Index: ", index, ", Element: ", element;
     }
+  }
+
+  datatype E<T> = Done | Next(T, () -> E<T>)
+
+  function OneTwoThree(): E<nat> {
+    Next(1, () => Next(2, () => Next(3, () => Done)))
+  }
+
+  function CountdownFrom(n: nat): E<nat> {
+    if n > 0 then
+      Next(n, () => CountdownFrom(n - 1))
+    else
+      Done
+  }
+
+  function CountupFrom(n: nat): E<nat> {
+    if n > 0 then
+      Next(n, () => CountdownFrom(n + 1))
+    else
+      Done
   }
 
   // iterator Iter<T(0)>(s: set<T>) yields (x: T)
