src/Enumeration/Loopers.dfy
@@ -24,21 +24,16 @@ module Loopers {
   }
 
   trait TerminatingLooper extends Validatable {
-    // Will need to be arbitrary termination clause somehow instead
+    // Would be better as an arbitrary termination clause somehow instead
     // https://github.com/dafny-lang/dafny/issues/762
-    // TODO: split up the ghost version from the version called at runtime?
-    // Implementor needs to use this to prove termination, but caller
-    // only needs Done()
-    function method Decreases(): nat
+    function Decreases(): nat
       reads Repr
       decreases Repr
       requires Valid()
     predicate method Done() 
       reads Repr
       requires Valid()
-    {
-      Decreases() == 0
-    }
+      ensures Decreases() == 0 ==> Done()
 
     method Step() 
       requires Valid()
@@ -55,9 +50,11 @@ module Loopers {
     ensures l.Valid()
     ensures l.Done()
   {
-    while (l.Decreases() > 0)
+    while (!l.Done())
       invariant l.Valid()
+      // Could this be a more general Ensures or Invariant?
       invariant fresh(l.Repr - old(l.Repr))
+      decreases l.Decreases()
     {
       l.Step();
     }
@@ -68,7 +65,10 @@ module Loopers {
     const elements: seq<T>
     var index: nat
 
-    constructor(s: seq<T>) {
+    constructor(s: seq<T>) 
+      ensures Valid()
+      ensures fresh(Repr - {this})
+    {
       elements := s;
       index := 0;
       Repr := {this};
@@ -83,11 +83,19 @@ module Loopers {
       && 0 <= index <= |elements|
     }
 
-    function method Decreases(): nat
+    function Decreases(): nat
       reads Repr
       requires Valid()
     {
       |elements| - index
+    }
+
+    predicate method Done() 
+      reads Repr
+      requires Valid()
+      ensures Decreases() == 0 ==> Done()
+    {
+      index == |elements|
     }
 
     method Step()
@@ -102,13 +110,33 @@ module Loopers {
     }
   }
 
-  class ForEach<T> extends TerminatingLooper {
+  // TODO: Some similarities between this and composing
+  // two Actions together.
+  // One is:
+  //   var r := action1.Invoke(a);
+  //   var r2 := action2.Invoke(r);
+  // Other is:
+  //   var r := looper.Step();
+  //   var _ := action.Invoke(r);
+  //   var r2 := looper.Step();
+  //   var _ := action.Invoke(r2);
+  //   ...
+  
+  class ForEach extends TerminatingLooper {
     const iter: TerminatingLooper
     const body: Action<TerminatingLooper, ()>
 
-    constructor(iter: TerminatingLooper, body: Action<TerminatingLooper, ()>) {
+    constructor(iter: TerminatingLooper, body: Action<TerminatingLooper, ()>)
+      requires iter.Valid()
+      requires body.Valid()
+      requires iter.Repr !! body.Repr
+      requires iter.Valid() ==> body.Requires(iter)
+      requires iter.Valid() ==> body.Modifies(iter) !! iter.Repr
+      ensures Valid()
+    {
       this.iter := iter;
       this.body := body;
+      Repr := {this} + iter.Repr + body.Repr;
     }
 
     predicate Valid() 
@@ -121,19 +149,28 @@ module Loopers {
       && ValidComponent(body)
       && iter.Repr !! body.Repr
       && (iter.Valid() ==> body.Requires(iter))
-      && (iter.Valid() ==> body.Modifies(iter) == {})
+      // TODO: This needs to be a forall somehow
+      && (iter.Valid() ==> body.Modifies(iter) !! iter.Repr)
     }
 
-    function method Decreases(): nat 
+    function Decreases(): nat 
       reads Repr
       requires Valid()
     {
       iter.Decreases()
     }
 
+    predicate method Done() 
+      reads Repr
+      requires Valid()
+      ensures Decreases() == 0 ==> Done()
+    {
+      iter.Done()
+    }
+
     method Step() 
       requires Valid()
-      requires Decreases() > 0
+      requires !Done()
       modifies Repr
       decreases Repr
       ensures ValidAndDisjoint()
@@ -141,11 +178,78 @@ module Loopers {
     {
       iter.Step();
       Repr := Repr + iter.Repr;
+
+      assert iter.Valid();
+      assert  this in Repr;
+      assert  ValidComponent(iter);
+      assert  ValidComponent(body);
+      assert  iter.Repr !! body.Repr;
+      assert  (iter.Valid() ==> body.Requires(iter));
+      assert  (iter.Valid() ==> body.Modifies(iter) !! iter.Repr);
+      assert Valid();
       
       var _ := body.Invoke(iter);
-      Repr := Repr +  body.Repr;
+      Repr := Repr + body.Repr;
     }
   }
 
-  
+  class SeqCollector<T> extends Action<T, ()> {
+
+    var elements: seq<T>
+
+    constructor() 
+      ensures Valid()
+      ensures fresh(Repr - {this})
+    {
+      elements := [];
+      Repr := {this};
+    }
+
+    predicate Valid() 
+      reads this, Repr 
+      ensures Valid() ==> this in Repr 
+      decreases Repr
+    {
+      && this in Repr
+    }
+
+    method Invoke(t: T) returns (nothing: ())
+      requires Valid()
+      requires Requires(t)
+      modifies Modifies(t)
+      decreases Decreases(t)
+      ensures ValidAndDisjoint()
+      ensures old(allocated(())) && Ensures(t, ())
+    {
+      elements := elements + [t];
+    }
+
+    predicate Requires(t: T) {
+      true
+    }
+
+    // Need this separately from Repr for callers
+    // Repr is the frame for Valid(), but callers
+    // need to know what ELSE gets modified.
+    function Modifies(t: T): set<object> requires Requires(t) {
+      {this}
+    }
+
+    function Decreases(t: T): nat {
+      0
+    }
+    
+    twostate predicate Ensures(t: T, nothing: ()) {
+      true
+    }
+  }
+
+
+  method Main() {
+    var numbers := [1, 2, 3, 4, 5];
+    var numbersIter := new SeqLooper(numbers);
+    var numbersPrinterLooper := new SeqCollector();
+    var forEachLoop := new ForEach(numbersIter, numbersPrinterLooper);
+    DoLoop(forEachLoop);
+  }
 }
